AP/AP/Bounded.lean
@@ -1,0 +1,156 @@
+import AP.AP.King
+
+namespace AP
+
+theorem State.length_hist_lt_of_tr {s s' p}
+(h : sys.tr s p = some s') : s.hist.length < s'.hist.length := by
+  simp [hist_eq_of_tr h]
+
+theorem State.forall_d_wins_bounded_of_forall_d_wins {s} [hs : sys.WF s]
+{d : DStrat} [Hd : d.WF] (h : ∀ (a : AStrat), a.WF → s.d_wins ⟨a, d⟩) :
+∃ (n : ℕ), ∀ (a : AStrat), a.WF → (sys.simulate (Strat.mk a d).f s n).2 ≠ 0 := by
+  contrapose! h
+  simp
+  apply exi_a_wins_of_ind (p := λ s => ∀ (n : ℕ), ∃ (a : AStrat), a.WF ∧
+    (sys.simulate (Strat.mk a d).f s n).2 = 0) h <;> clear! s; rotate_left
+  · intro sd hd sa ih h₁ n
+    specialize ih (n + 1)
+    obtain ⟨a, Ha, ih⟩ := ih
+    simp [h₁] at ih
+    use a
+  intro sa ha ih
+  have ht : sys.hasTr sa
+  · specialize ih 1
+    obtain ⟨a, h₁, h₂⟩ := ih
+    simp at h₂; split at h₂; simp at h₂; nm x sd h₃; clear x
+    exact ⟨_, _, h₃⟩
+  rw [skolemize'] at ih
+  obtain ⟨f, hf⟩ := ih
+  obtain ⟨g, hg⟩ : ∃ (g : ℕ → {pa : PointZ // pa.dist sa.aPos ≤ sa.pw}),
+    ∀ n, n ≠ 0 → (g n).1 = (f n).f sa
+  · refine' ⟨_, _⟩
+    · intro n
+      use if n = 0 then sa.aPos else (f n).f sa
+      specialize hf n
+      rcases hf with ⟨h₁, h₂⟩
+      cases n <;> simp; nm n
+      simp at h₂; split at h₂; simp at h₂; nm x sd h₃; clear x
+      simp at h₃
+      exact h₃.1.2.2
+    intro n hn
+    simp [hn]
+  have h₂ := @Point.finite_setOf_dist_le sa.aPos sa.pw
+  obtain ⟨⟨pa, h₃⟩, h₄⟩ := Set.exists_infinite_preimage_of (f := g) (hb := h₂)
+  simp at h₃
+  suffices h₅ : ∀ n, n ≠ 0 → ∃ (a : AStrat), a.WF ∧ a.f sa = pa ∧
+    (sys.simulate (Strat.mk a d).f sa n).2 = 0
+  · obtain ⟨a, h₆, h₇, h₈⟩ := h₅ 1 (by simp)
+    clear h₈
+    obtain ⟨sd, h₈⟩ := a.validTr ht
+    rw [h₇] at h₈; clear h₇
+    use pa, sd, h₈
+    clear! a
+    intro n
+    specialize h₅ (n + 1) (by simp)
+    obtain ⟨a, Ha, h₅, h₆⟩ := h₅
+    simp [h₅, h₈] at h₆
+    use a
+  suffices h₅ : ∀ (k : ℕ), ∃ (n : ℕ), k ≤ n ∧ g n = ⟨pa, h₃⟩
+  · intro k hk
+    specialize h₅ k
+    obtain ⟨n, hn, h₅⟩ := h₅
+    specialize hg n _
+    · rintro rfl; simp [hk] at hn
+    rw [Subtype.ext_iff, hg] at h₅
+    specialize hf n
+    rcases hf with ⟨hf, h₆⟩
+    use f n, hf, h₅
+    exact System.simulate_snd_eq_zero_of_le_and_eq_zero h₆ hn
+  contrapose! h₄
+  simp [Set.preimage]
+  obtain ⟨k, hk⟩ := h₄
+  apply Set.finite_of_subset_finset # Finset.Ico 0 k
+  simp
+  intro n h₄
+  specialize hk n
+  simp [h₄] at hk
+  exact hk
+
+theorem State.forall_d_wins_iff_forall_d_wins_bounded {s} [hs : sys.WF s]
+{d : DStrat} [Hd : d.WF] : (∀ (a : AStrat), a.WF → s.d_wins ⟨a, d⟩) ↔
+∃ (n : ℕ), ∀ (a : AStrat), a.WF → (sys.simulate (Strat.mk a d).f s n).2 ≠ 0 := by
+  use forall_d_wins_bounded_of_forall_d_wins
+  rintro ⟨n, h₁⟩
+  intro a Ha
+  specialize h₁ a Ha
+  use n
+
+theorem State.d_hws_iff_d_hws_bounded {s} [hs : sys.WF s]
+(h : s.d_hws) : ∃ (n : ℕ) (d : DStrat), d.WF ∧ ∀ (a : AStrat), a.WF →
+(sys.simulate (Strat.mk a d).f s n).2 ≠ 0 := by
+  obtain ⟨d, Hd, h⟩ := h
+  rw [forall_d_wins_iff_forall_d_wins_bounded] at h
+  obtain ⟨n, h₁⟩ := h
+  use n, d
+
+def State.getATrap (s : State) : Set PointZ :=
+  {p | ∃ s', sys.Reachable s s' ∧ s'.aPos = p}
+
+def State.aTrapped (s : State) : Prop :=
+  s.getATrap.Finite
+
+theorem State.a_wins_iff_add {s st} (k : ℕ) :
+s.a_wins st ↔ ∀ n, (sys.simulate st.f s # k + n).2 = 0 := by
+  constructor <;> intro h₁ n
+  · exact h₁ # k + n
+  · apply System.simulate_snd_eq_zero_of_le_and_eq_zero # h₁ n
+    linarith
+
+theorem State.d_wins_iff_add {s st} (k : ℕ) :
+s.d_wins st ↔ ∃ n, (sys.simulate st.f s # k + n).2 ≠ 0 := by
+  constructor <;> rintro ⟨n, h₁⟩
+  · use n
+    contrapose! h₁
+    apply System.simulate_snd_eq_zero_of_le_and_eq_zero h₁
+    linarith
+  · use k + n
+
+#check 0 #exit
+
+not_reachable_of_acyclic_and_simulate_and_lt
+
+theorem State.d_hws_of_exi_aTrapped {s} [hs : sys.WF s]
+(h : ∃ (d : DStrat), d.WF ∧ ∀ (a : AStrat), a.WF → ∃ n,
+(sys.simulate (Strat.mk a d).f s n).1.aTrapped) : s.d_hws := by
+  classical
+  obtain ⟨d, Hd, h₁⟩ := h
+  rw [←not_a_hws_iff, a_hws]
+  push_neg; simp
+  intro a Ha
+  specialize h₁ a Ha
+  obtain ⟨n, h₁⟩ := h₁
+  generalize hr : sys.simulate (Strat.mk a d).f s n = r
+  rcases r with ⟨s₁, r⟩
+  simp [hr] at h₁
+  generalize hd₁ : DStrat.mk' (λ s => if sys.Reachable s₁ s then
+    choose? (· ∈ s.getATrap) else d.f s) = d₁
+  have Hd₁ : d₁.WF; subst hd₁; infer_instance
+  
+  by_cases hr' : r = 0; rotate_left
+  · use d, Hd, n; simpa [hr]
+  subst hr'
+  
+  use d₁, Hd₁
+  use n + s₁.getATrap.ncard
+  have h₂ : sys.simulate (Strat.mk a d₁).f s n = ⟨s₁, 0⟩
+  · rw [←hr]
+    apply simulate_congr # by simp
+    rintro k hk sd hd h₂ h₃ ⟨pd, sa, h₄⟩
+    dsimp
+    suffices h₅ : ¬sys.Reachable s₁ sd
+    · simp [←hd₁, mk_strat_fn, h₅]
+    have h₅ := System.reachable_of_simulate_full h₂
+    have h₆ : sys.Reachable sa s₁
+    · 
+  simp [System.simulate_add, h₂]
+  sorry
